---
layout: math
title: Bijections
nav_order: 3
mathjax: true
parent: Computability
---

# Bijections

* A function $f : A \to B$ is __injective__ (or 1-1) just if for any $a_1, a_2
\in A$ we have that $f(a_1) = f(a_2)$ implies $a_1 = a_2$.

* A function $f : A \to B$ is __surjective__ just if for any $b \in B$ there
exists $a \in A$ such that $f(a) = b$.

* A function $f : A \to B$ is a __bijection__ just if it is injective and
surjective.

# Inverses

Let $f : A \to B$ be a function.

$f$ has an __inverse__ just if there exists a function $f^{-1} : B \to A$
such that
* for all $a \in A$ we have $f^{-1}(f(a)) = a$
* for all $b \in B$ we have $f(f^{-1}(b)) = b$

Both equations are necessary!

Using [function
composition](https://uob-coms20007.github.io/reference/prereqs/functions.html#composition)
and the [identity
function](https://uob-coms20007.github.io/reference/prereqs/functions.html#identity-function),
they may be re-written in a so-called _point-free_ style as
* $f^{-1} \circ f = \textsf{id}_A$
* $f \circ f^{-1} = \textsf{id}_B$

In the problem sheet you will prove the following result.

*Claim.* A function $f : A \to B$ is a bijection if and only if it has an inverse.

Thus, a bijection $f : A \to B$ is a device for putting the sets $A$ and $B$
into perfect correspondence: it maps every $a \in A$ to a uniquely associated
$b \in B$. 
# Integers vs. natural numbers

In light of this, the following result is a bit surprising.

Define

$$
\begin{aligned}
  &\beta : \mathbb{Z} \to \mathbb{N} \\
  &\beta(x) = \begin{cases}
    2x    & \text{ if $x \geq 0$} \\
    -2x-1 & \text{ otherwise}
  \end{cases}
\end{aligned}
$$

$\beta$ maps 
* positive numbers to even numbers
* negative numbers to odd numbers

*Claim.* The function $\beta$ is a bijection.

_Proof._ 

1. $\beta$ is injective. Let $k_1, k_2 \in \mathbb{Z}$, and suppose $f(k_1) = f(k_2)$.
   There are four cases to consider:
   * *$k_1, k_2$ both positive.* Then $f(k_1) = f(k_2)$ is exactly the statement that $2k_1 = 2k_2$, whence $k_1 = k_2$.
   * *$k_1, k_2$ both negative.* Then $f(k_1) = f(k_2)$ is exactly the statement that $-2k_1 - 1 = -2k_2 - 1$, whence $k_1 = k_2$.
   * *$k_1$ positive, $k_2$ negative.* Then $f(k_1) = f(k_2)$ is exactly the statement that $2k_1 = -2k_2 - 1$. From this we infer $k_1 + k_2 = -1/2$, which cannot happen as both are whole numbers. Thus, this case cannot occur in practice, so there is nothing to prove.
   * *$k_1$ negative, $k_2$ positive.* Similar to the last case.

2. $\beta$ is surjective. Let $n \in \mathbb{N}$. We consider the parity of $n$.
   * If $n$ is even, write it as $n = 2n'$. Then $f(n') = 2n' = n$.
   * If $n$ is odd, write it as $n = 2n' + 1$. Then $f(-n' - 1) = -2(-n' - 1) - 1 = 2n' + 1$.

Hence $\beta$ is a bijection. â–£